\documentclass[a4paper,10pt]{extarticle}
\usepackage{amsmath,amsthm,amssymb}
\usepackage[linkcolor=Blue, urlcolor=Blue,colorlinks=true]{hyperref}
\usepackage[usenames,dvipsnames]{xcolor}							% Fancy colors
\usepackage{fullpage}
\usepackage{enumitem}
\usepackage{soul}

% Macros
\newcommand{\ii}{\textup{i}}									% \textup{i} := \sqrt{-1}
\newcommand{\bb}[1]{\mathbb{#1}}								% Blackboard boldface for R, C, N, Q
\newcommand{\inv}[1]{{#1}^{-1}}								% Inverse

\title{403_PS8}
\author{Ben Clark}
\date{March 2018}

\begin{document}


\section{Introduction}

Let 

\[ f = \sum_{k=0}^{n} a_k x^k\] and 
\[ g = \sum_{k=0}^{m} b_k x^k\]

then without loss of generality assume that $n >= m$, so

\begin{align*}
    (f + g)' &= ((\sum_{k=0}^{n} a_k x^k) + (\sum_{k=0}^{m} b_k x^k))' \\
    &= (\sum_{k=0}^{n} a_k x^k + b_k x^k)' \\
    &= (\sum_{k=0}^{n} (a_k + b_k) x^k)' \\
    &= \sum_{k=0}^{n - 1} (k+1)(a_{k+1} + b_{k+1}) x^k \\
    &= \sum_{k=0}^{n - 1} (((k+1) a_{k+1}) + ((k+1) b_{k+1})) x^k \\
    &= \sum_{k=0}^{n - 1} ((k+1) a_{k+1} x^k) + ((k+1) b_{k+1} x^k ) \\
    &= \sum_{k=0}^{n - 1} ((k+1) a_{k+1} x^k) + \sum_{k=0}^{n - 1} ((k+1) b_{k+1} x^k ) \\
    &= \sum_{k=0}^{n - 1} ((k+1) a_{k+1} x^k) + \sum_{k=0}^{m - 1} ((k+1) b_{k+1} x^k ) \\
    &= f' + g'
\end{align*}

\end{document}
